proof that thread is active

src/rel_hoare.lean
@@ -50,6 +50,12 @@ def initial_kernel_assertion_left_thread_state {init₁ : ℕ → σ₁} {init�
 
 #check initial_kernel_assertion_left_thread_state
 
+def initial_kernel_assertion.left_all_threads_active {init₁ : ℕ → σ₁} {init₂ : ℕ → σ₂} {P : memory τ₁ → memory τ₂ → Prop} 
+{f₁ : memory τ₁ → ℕ} {f₂ : memory τ₂ → ℕ} {m₁ : memory τ₁} {m₂ : memory τ₂} 
+{n₁} {s₁ : state n₁ σ₁ τ₁} {ac₁ : vector bool n₁} {n₂} {s₂ : state n₂ σ₂ τ₂} {ac₂ : vector bool n₂}
+(i : initial_kernel_assertion init₁ init₂ P f₁ f₂ m₁ m₂ n₁ s₁ ac₁ n₂ s₂ ac₂) := i.right.right.right.right.right.right.right.left
+
+#check initial_kernel_assertion.left_all_threads_active
 
 lemma rel_kernel_to_program (k₁ : kernel σ₁ τ₁) (k₂ : kernel σ₂ τ₂) (init₁ : ℕ → σ₁) (init₂ : ℕ → σ₂) (P Q : memory τ₁ → memory τ₂ → Prop) (f₁ : memory τ₁ → ℕ) (f₂ : memory τ₂ → ℕ)
  (h : {* λ n₁ s₁ ac₁ n₂ s₂ ac₂, ∃ m₁ m₂, initial_kernel_assertion init₁ init₂ P f₁ f₂ m₁ m₂ n₁ s₁ ac₁ n₂ s₂ ac₂ *} k₁ ~ k₂ 
